\begin{equation}
	\begin{split}
	Pr[a_\ell\ \textrm{is the final}\ s]\ 
	& = Pr[a_\ell\ \textrm{is chosen as}\ s\ \cdot \prod_{i=\ell+1}^{m} Pr[a_i\ \textrm{does not replace}\ a_\ell\ \textrm{as}\ s] \\
	& = \frac{1}{\ell} \cdot \prod_{i=\ell+1}^{m}\left(1-\frac{1}{i}\right) \\
	& = \frac{1}{\ell} \cdot \prod_{i=\ell+1}^{m}\frac{1-i}{i} \\
	& = \frac{1}{m}
	\end{split}
\end{equation}

\begin{equation}
	\begin{split}
	Pr[a_{\ell_1}, a_{\ell_2}\ \textrm{form the final sample}]\ 
	& = \frac{2}{\ell_2} \cdot \prod_{\ell_1<i<\ell_2} \left(1- \frac{2}{i} + \frac{2}{i} \cdot \frac{1}{2}\right) \cdot \frac{2}{\ell_2} \cdot \frac{1}{2} \cdot \prod_{\ell_2 < j \le m} \left( 1 - \frac{2}{j} \right)  \\
	& = \frac{2}{\ell_1 \cdot \ell_2} \cdot \prod_{\ell_1 < i < \ell_2} \frac{i-1}{i} \cdot \prod_{\ell_2 < j \le m} \frac{j-2}{j} \\
	& = \frac{2}{\left( m - 1 \right) \cdot m} \\
	& = 1\Big/\tbinom{m}{2}
	\end{split}
\end{equation}

